updating globals initialization

coq/Concrete.v
@@ -538,9 +538,7 @@ Fixpoint init_global_store_internal (gs : dv_store) (l : list llvm_global) : opt
   end
 .
 
-Definition init_global_store (m : llvm_module) : option dv_store :=
-  init_global_store_internal empty_dv_store (m_globals m)
-.
+Definition init_global_store (m : llvm_module) : option dv_store := Some empty_dv_store.
 
 (* TODO: assumes that there are no parameters *)
 Definition init_state (m : llvm_module) (d : llvm_definition) : option state :=
